

1. (24 pts) Let $X_1, \dots, X_n \stackrel{\text{iid}}{\sim} \text{Gamma}(\alpha, \beta)$.
- (a) (6 pts) Find a sufficient statistic for the parameter β , assuming α is known. Is the statistic you found above minimally sufficient? Justify your answer.
 - (b) (6 pts) Find the MLE of β assuming α is known.
 - (c) (6 pts) Find the Fisher information and construct an approximate 95% normal-based confidence interval for β .
 - (d) (6 pts) Find the asymptotic distribution for the MLE of β assuming α is known.

Solution:

- (a) Assume α is known.

$$\begin{aligned} f(x_1, \dots, x_n; \beta) &= \prod_{i=1}^n \frac{\beta^\alpha}{\Gamma(\alpha)} X_i^{\alpha-1} e^{-\beta X_i} \\ &= \underbrace{\prod_{i=1}^n X_i^{\alpha-1}}_{h(\mathbf{x})} \underbrace{\left(\frac{\beta^\alpha}{\Gamma(\alpha)} \right)^n \exp\left(-\beta \sum_{i=1}^n X_i\right)}_{g(T(\mathbf{x}), \beta)}. \end{aligned}$$

Therefore a sufficient statistic for β is $\sum_{i=1}^n X_i$. For minimal sufficiency using the exponential family form:

$$f(x_1, \dots, x_n; \beta) = \underbrace{\left[\prod_{i=1}^n X_i^{\alpha-1} \right]}_{h(\mathbf{x})} [\Gamma(\alpha)]^{-n} \exp \left(\underbrace{-\beta \sum_{i=1}^n X_i}_{\eta_1(\beta)} + \underbrace{\alpha n \log \beta}_{A(\beta)} \right).$$

Thus, $\sum_i X_i$ is minimally sufficient.

- (b)

$$\begin{aligned} \frac{\partial f(x_1, \dots, x_n; \beta)}{\partial \beta} &= \frac{\log(\prod_{i=1}^n X_i^{\alpha-1}) + n\alpha \log \beta - n \log(\Gamma(\alpha)) - \beta \sum_{i=1}^n X_i}{\partial \beta} \\ &= \frac{n\alpha}{\beta} - \sum_{i=1}^n X_i. \end{aligned}$$

Setting equal to 0 and solving yields

$$\hat{\beta}_{MLE} = \frac{n\alpha}{\sum_i X_i}.$$

The second derivative is

$$\frac{\partial^2 f(x_1, \dots, x_n; \beta)}{\partial \beta^2} = -\frac{n\alpha}{\beta^2} < 0.$$

(c) First, find the Fisher information.

$$\begin{aligned} I(\beta) &= -E_\beta \left[\frac{\partial^2}{\partial \beta^2} \log f(x; \beta) \right] \\ &= -E_\beta \left[\frac{\partial^2}{\partial \beta^2} \log \left(\frac{\beta^\alpha}{\Gamma(\alpha) x^{\alpha-1} e^{-\beta x}} \right) \right] \\ &= -E_\beta \left[\frac{\partial}{\partial \beta} \left(\frac{\alpha}{\beta} - x \right) \right] \\ &= -E_\beta \left[-\frac{\alpha}{\beta^2} \right] = \frac{\alpha}{\beta^2}. \end{aligned}$$

The asymptotic distribution is thus

$$\begin{aligned} \sqrt{n}(\hat{\beta}_{MLE} - \beta) &\rightarrow N(0, 1/I_1(\beta)) \\ \Rightarrow \sqrt{n} \left(\frac{n\alpha}{\sum_{i=1}^n X_i} - \beta \right) &\rightarrow N(0, \hat{\beta}_{MLE}^2/\alpha). \end{aligned}$$

An approximate 95% confidence interval is

$$\left| \frac{\sqrt{n}(\frac{n\alpha}{\sum_i X_i} - \beta)}{\sqrt{\frac{\hat{\beta}_{MLE}^2}{\alpha}}} \right| > z_{0.025}.$$

(d) The asymptotic distribution for the MLE of β assuming α is known is

$$\frac{\hat{\beta}_{MLE} - \beta}{\sqrt{\frac{\hat{\beta}_{MLE}^2}{\alpha}}} \rightarrow N(0, 1)$$

or equivalently

$$\hat{\beta}_{MLE} \rightarrow N \left(\beta, \frac{n\alpha}{(\sum_{i=1}^n X_i)^2} \right)$$

or

$$\hat{\beta}_{MLE} \rightarrow N \left(\beta, \sqrt{\frac{\beta^2}{n\alpha}} \right).$$

2. (12 pts) Let X and Y be two random variables with joint distribution F . Suppose we observe pairs $(x_1, y_1), \dots, (x_n, y_n)$, a random sample from F .
- (a) (6 pts) Without making any assumptions about F , form a statistic for testing $H_0 : P(X > Y) = 0.5$.
- (b) (6 pts) How would you calculate the p-value?

Solution:

- (a) Let $Z = X - Y$. Then $Z_i = X_i - Y_i$ for $i = 1, \dots, n$. Let

$$B = \sum_{i=1}^n I(Z_i > 0) =: \sum_{i=1}^n b_i$$

where $B \sim \text{Bin}(n, p)$ and $p = P(Z > 0)$. Then $H_0 : p = 0.5$. For B , we know that the MLE for p is

$$\hat{p} = \frac{\sum_{i=1}^n I(Z_i > 0)}{n}.$$

The Wald test gives

$$\frac{\hat{p} - 0.5}{\hat{se}(\hat{p})} \rightarrow N(0, 1).$$

We also know that

$$\hat{se}(\hat{p}) = \hat{se}\left(\frac{\sum_{i=1}^n I(Z_i > 0)}{n}\right) = \hat{se}\left(\frac{B}{n}\right) = \sqrt{\frac{\hat{p}(1 - \hat{p})}{n}}.$$

Therefore, a test statistic is

$$\left| \frac{\hat{p} - 0.5}{\sqrt{\frac{\hat{p}(1 - \hat{p})}{n}}} \right|.$$

- (b) First, we should calculate the number of pairs (X_i, Y_i) , where $X_i > Y_i$. Let that number be N . Then the p-value is given by

$$\sup_{\theta \in \Theta_0} P_{\theta}(T(B) \geq T(b))$$

where

$$T(B) = \left| \frac{\hat{p} - 0.5}{\sqrt{\frac{\hat{p}(1-\hat{p})}{n}}} \right| \quad T(b) = \left| \frac{\frac{N}{n} - 0.5}{\sqrt{\frac{\frac{N}{n}(1-\frac{N}{n})}{n}}} \right|$$

and we know that under H_0 , $T(B) \rightarrow N(0, 1)$. Therefore, the p-value is $2(1 - \Phi(T(b)))$.

3. (6 pts) Let $X_1, \dots, X_n \stackrel{\text{iid}}{\sim} \mathcal{N}(u, 1)$ and let $Y_1, \dots, Y_n \stackrel{\text{iid}}{\sim} \mathcal{N}(v, 4)$. X_i 's and Y_i 's are independent of each other. Find the Fisher information matrix for the parameter (u, v) .

Solution:

$$\mathcal{L}_n(X, Y; u, v) = \prod_{i=1}^n (2\pi)^{-1/2} \exp\left(-\frac{1}{2}(X_i - u)^2\right) \prod_{i=1}^n (8\pi)^{-1/2} \exp\left(-\frac{1}{8}(Y_i - v)^2\right).$$

$$\ell_n(X, Y; u, v) = -\frac{1}{2} \log 2\pi - \frac{1}{2} \sum_{i=1}^n (X_i - u)^2 - \frac{1}{2} n \log 8\pi - \frac{1}{8} \sum_{i=1}^n (Y_i - v)^2.$$

$$\frac{\partial \ell_n}{\partial u} = \sum_{i=1}^n (X_i - u)$$

$$\frac{\partial \ell_n}{\partial v} = \frac{1}{4} \sum_{i=1}^n (Y_i - v)$$

$$\frac{\partial^2 \ell_n}{\partial u^2} = \sum_{i=1}^n (-1) = -n$$

$$\frac{\partial^2 \ell_n}{\partial u \partial v} = \frac{\partial^2 \ell_n}{\partial v \partial u} = 0$$

$$\frac{\partial^2 \ell_n}{\partial v^2} = \frac{1}{4} \sum_{i=1}^n (-1) = -\frac{1}{4}n.$$

Thus the Fisher information matrix is given by

$$\begin{pmatrix} n & 0 \\ 0 & \frac{1}{4}n \end{pmatrix}.$$

4. (12 pts) (Cont'd with problem 3.) Now we consider a Bayesian setting. Let $X_1, \dots, X_n \stackrel{\text{iid}}{\sim} \mathcal{N}(u, 1)$ and let $Y_1, \dots, Y_n \stackrel{\text{iid}}{\sim} \mathcal{N}(v, 4)$. X_i 's and Y_i 's are independent of each other.

- (a) (6 pts) Assume the conjugate prior distribution for u is $\mathcal{N}(a, b)$. Find the posterior distribution for u , conditioning on X_1, \dots, X_n . It is fine to write the distribution family and specify the parameters; you do not need to write out the PDF or CDF.
- (b) (6 pts) Suppose we use squared error loss, and let \hat{u}_n be the Bayes estimator based on observing X_1, \dots, X_n . Find \hat{u}_n .

Solution:

(a)

$$\begin{aligned}
 f(u \mid X_1, \dots, X_n) &\propto f(X_1, \dots, X_n \mid u) f(u) \\
 &= \prod_{i=1}^n (2\pi)^{-1/2} \exp\left(-\frac{1}{2}(X_i - u)^2\right) \cdot (2\pi b)^{-1/2} \exp\left(-\frac{1}{2b}(u - a)^2\right) \\
 &\propto \exp\left(-\frac{1}{2} \sum_{i=1}^n (X_i - u)^2 - \frac{1}{2b}(u - a)^2\right) \\
 &= \exp\left(-\frac{b \sum_i X_i^2 - 2bu \sum_i X_i + nbu^2 + u^2 + a^2 - 2ua}{2b}\right) \\
 &\propto \exp\left(-\frac{(nb + 1)u^2 - 2(a + b \sum_i X_i)u}{2b}\right) \\
 &\propto \exp\left(-\frac{\left(u - \frac{a + b \sum_i X_i}{nb + 1}\right)^2}{2 \frac{b}{nb + 1}}\right)
 \end{aligned}$$

Therefore,

$$u \mid X_1, \dots, X_n \sim N\left(\frac{a + b \sum_{i=1}^n X_i}{nb + 1}, \frac{b}{nb + 1}\right).$$

(b) The Bayes risk is

$$r(f, \hat{u}) = E_X[r(\hat{u} \mid X^n)] = \int r(\hat{u} \mid x) f(x) dx.$$

For every X^n , $r(\hat{u} \mid X^n)$ gives a single value so if we need to minimize Bayes risk, we just need to minimize $r(\hat{u} \mid X^n)$ for every X^n . Under squared error loss, the posterior mean minimizes $r(\hat{u} \mid X^n)$ so

$$\hat{u}_n = \frac{a + b \sum_{i=1}^n X_i}{nb + 1}.$$

5. (24 pts + 10 pts (extra)) Consider the regression model $Y_i = r(X_i) + \varepsilon_i$ for $i = 1, \dots, n$, with $\varepsilon_1, \dots, \varepsilon_n$ iid and $\varepsilon_i \sim \mathcal{N}(0, \sigma^2)$.
- (a) (6 pts) Consider X_1, \dots, X_n as given. Find a Kernel estimator for $r(x)$. Specify what kernel function you use.
 - (b) (10 pts) (Optional; for extra credit) Cont'd with (a). Is the above estimator unbiased at a given x ? What is the variance of the above estimator at a given x ? Explain the tradeoff between bias and variance.
 - (c) (6 pts) Now consider X_1, \dots, X_n as given and $r(X_i) = X_i$. Find the MLE for σ .
 - (d) (6 pts) Cont'd with (c). What is the MLE's asymptotic distribution? Approximate asymptotic variance?
 - (e) (6 pts) Cont'd with (c). Now we assume that $n = 2m$, $\varepsilon_i \sim \mathcal{N}(0, \sigma_1^2)$ when $i = 1, \dots, m$, and $\varepsilon_i \sim \mathcal{N}(0, \sigma_2^2)$ when $i = m+1, \dots, 2m$. Carry out a test for testing $H_0 : \sigma_1 = \sigma_2$ vs. $H_1 : \sigma_1 \neq \sigma_2$.

Solution:

- (a) A kernel estimator is given by

$$\hat{r}(x) = \frac{\sum_{j=1}^n w_j(x) Y_j}{\sum_{i=1}^n w_i(x)}$$

where $w_j(x) = K(\frac{x-X_j}{n})$ is a kernel for example $w_j(x) = \exp\{-\left(\frac{x-X_j}{n}\right)^2\}$.

- (b)

- (c)

$$\begin{aligned} f(y_1, \dots, y_n; \sigma) &= \prod_{i=1}^n \frac{1}{\sqrt{2\pi\sigma^2}} \exp\left(-\frac{1}{2\sigma^2}(y_i - r(x_i))^2\right) \\ &= \left(\frac{1}{\sqrt{2\pi\sigma^2}}\right)^n \exp\left(-\frac{1}{2\sigma^2} \sum_{i=1}^n (y_i - x_i)^2\right). \end{aligned}$$

The log-likelihood is then given by

$$\ell(\theta) = C - n \log \sigma - \frac{1}{2\sigma^2} \sum_{i=1}^n (y_i - x_i)^2$$

with derivative

$$\frac{\partial \ell(\theta)}{\partial \sigma} = -\frac{n}{\sigma} + \frac{\sum_{i=1}^n (y_i - x_i)^2}{\sigma^3}.$$

Setting equal to 0 and solving gives

$$\hat{\sigma}_{MLE}^2 = \frac{\sum_{i=1}^n (y_i - x_i)^2}{n}$$

and by equivariance,

$$\hat{\sigma}_{MLE} = \sqrt{\frac{\sum_{i=1}^n (y_i - x_i)^2}{n}}.$$

We can check that the second derivative is negative:

$$\frac{\partial^2 \ell(\theta)}{\partial \sigma^2} = \frac{n}{\sigma^2} - \frac{3 \sum_{i=1}^n (y_i - x_i)^2}{\sigma^4} = \frac{n\sigma^2 - 3 \sum_{i=1}^n (y_i - x_i)^2}{\sigma^4} < 0.$$

- (d) We can use the Fisher information to compute the asymptotic distribution and variance.

$$\begin{aligned} I_n(\hat{\sigma}_{MLE}) &= -E_{\theta} \left[\frac{\partial^2}{\partial \theta^2} \ell_n(\theta) \right] \\ &= -E \left[\frac{n}{\sigma^2} - \frac{3 \sum_{i=1}^n (y_i - x_i)^2}{\sigma^4} \right] \\ &= -\frac{n}{\sigma^2} + \frac{3n\sigma^2}{\sigma^4} \\ &= \frac{2n}{\sigma^2}. \end{aligned}$$

Thus, the variance is

$$\text{Var}(\hat{\sigma}_{MLE}) = \frac{1}{I_n(\hat{\sigma}_{MLE})} = \frac{\sigma^2}{2n},$$

$$\hat{\text{Var}}(\hat{\sigma}_{MLE}) = \frac{1}{I_n(\hat{\sigma}_{MLE})} = \frac{\hat{\sigma}_{MLE}^2}{2n}.$$

and the asymptotic distribution is

$$\frac{\hat{\sigma}_{MLE} - \sigma}{\hat{se}(\hat{\sigma}_{MLE})} \rightarrow N(0, 1).$$

(e) We can perform a likelihood ratio test.

$$T(\mathbf{x}) = \frac{\sup_{\theta \in \Theta} L_n(\theta)}{\sup_{\theta \in \Theta_0} L_n(\theta)} = \frac{\sup_{\theta \in \Theta} L_n(\theta)}{L_n(\hat{\theta}_{\text{MLE}})} = \frac{L_n(\hat{\sigma}_{1,\text{MLE}}, \hat{\sigma}_{2,\text{MLE}})}{L_n(\hat{\sigma}_{\text{MLE}})}.$$

Under $H_0 : \sigma_1 = \sigma_2 = \sigma$.

$$\hat{\sigma}_{1,\text{MLE}} = \sqrt{\frac{1}{m} \sum_{i=1}^m (y_i - x_i)^2}, \quad \hat{\sigma}_{2,\text{MLE}} = \sqrt{\frac{1}{m} \sum_{i=m+1}^{2m} (y_i - x_i)^2},$$

$$\hat{\sigma}_{\text{MLE}} = \sqrt{\frac{1}{n} \sum_{i=1}^n (y_i - x_i)^2}.$$

Then, we can compute the test statistic

$$\begin{aligned} T(X) &= \frac{\left(\frac{1}{\hat{\sigma}_{1,\text{MLE}}} \cdot \frac{1}{\hat{\sigma}_{2,\text{MLE}}}\right)^m}{\left(\frac{1}{\hat{\sigma}_{\text{MLE}}}\right)^n} \exp\left(-\frac{1}{2\hat{\sigma}_{1,\text{MLE}}^2} \sum_{i=1}^m (y_i - x_i)^2 - \frac{1}{2\hat{\sigma}_{2,\text{MLE}}^2} \sum_{i=m+1}^{2m} (y_i - x_i)^2\right. \\ &\quad \left. + \frac{1}{2\hat{\sigma}_{\text{MLE}}^2} \sum_{i=1}^n (y_i - x_i)^2\right) \\ &= \frac{\hat{\sigma}_{\text{MLE}}^n}{(\hat{\sigma}_{1,\text{MLE}} \hat{\sigma}_{2,\text{MLE}})^m} \exp\left(-\frac{m}{2} - \frac{m}{2} + \frac{n}{2}\right) \\ &= \frac{\hat{\sigma}_{\text{MLE}}^n}{(\hat{\sigma}_{1,\text{MLE}} \hat{\sigma}_{2,\text{MLE}})^m}. \end{aligned}$$

The asymptotic distribution is given by

$$\Lambda(\mathbf{x}) = 2 \log T(\mathbf{x}) \sim \chi_1^2.$$

Reject H_0 if $\Lambda(\mathbf{x}) > \chi_{1,1-\alpha}^2$.

6. (12 pts) Suppose X_1, \dots, X_n are i.i.d. Poisson variables with mean λ and we are interested in estimating $p = P(X_i = 0) = e^{-\lambda}$.
- (a) (6 pts) One estimator for p is the proportion of zeros in the sample, $\tilde{p} = \#\{i \leq n : X_i = 0\}/n$. Find the limiting distribution for $\sqrt{n}(\tilde{p} - p)$.
- (b) (6 pts) Another estimator would be the maximum likelihood estimator \hat{p} . Give a formula for \hat{p} and determine the limiting distribution for $\sqrt{n}(\hat{p} - p)$.

Solution:

- (a) Note that \tilde{p} is the average of iid Bernoullis with success probability p . Then by the central limit theorem,

$$\sqrt{n}(\tilde{p} - p) \sim \mathcal{N}(0, \bar{\sigma}^2)$$

with some variance $\bar{\sigma}^2$. What variance? Simply the variance of each Bernoulli variate, so

$$\bar{\sigma}^2 = p(1 - p) = e^{-\lambda}(1 - e^{-\lambda}).$$

- (b) We may recall that the Poisson MLE is $\hat{\lambda} = \bar{X}$. (Of course, we can also derive it, but this has been done many times by now.) Then, by equivariance,

$$\hat{p} = e^{-\hat{\lambda}}.$$

By standard MLE theorems (or the central limit theorem), we also have

$$\sqrt{n}(\hat{\lambda} - \lambda) \sim \mathcal{N}(0, \gamma^2)$$

with some variance γ^2 . What variance? You can use either the CLT or the MLE theorems. If you use the CLT, then $\gamma^2 = \text{Var}(X_1) = \lambda$, the variance of a single Poisson. On the other hand, the MLE theorem for iid data says $\gamma^2 = 1/I_1(\lambda)$, the inverse Fisher information of one observation. We can compute

$$I_1(\lambda) = -\mathbb{E}[\ell_1''(\lambda)] = -\mathbb{E}\left[-\frac{X}{\lambda^2}\right] = \frac{\mathbb{E}[X]}{\lambda^2} = \frac{\lambda}{\lambda^2} = \frac{1}{\lambda},$$

so again $\gamma^2 = \lambda$.

Finally, by the delta method, we have

$$\sqrt{n}(\hat{p} - p) \sim \mathcal{N}(0, \sigma^2)$$

with some variance σ^2 . What variance? This is given by the delta method formula. Let $f(x) = e^{-x}$. Then $p = f(\lambda)$ and $\hat{p} = f(\hat{\lambda})$, and since $f'(\lambda) = -e^{-\lambda} = -p$, we can write

$$\sqrt{n}(\hat{p} - p) = \sqrt{n}(f(\hat{\lambda}) - f(\lambda)) \xrightarrow{d} \mathcal{N}(0, (f'(\lambda))^2 \cdot \lambda) = \mathcal{N}(0, \lambda e^{-2\lambda}) = \mathcal{N}(0, \lambda p^2),$$

showing us that $\sigma^2 = \lambda p^2 = \log(1/p) \cdot p^2$.

7. (10 pts) Consider a decision problem with possible states of nature θ_1 and θ_2 . Let X be a random variable with probability function $p(x | \theta)$:

$$P(X = 0 | \theta_1) = 0.2, P(X = 1 | \theta_1) = 0.8; P(X = 0 | \theta_2) = 0.4, P(X = 1 | \theta_2) = 0.6.$$

Two non-randomized actions a_1 and a_2 are considered with the following loss function:

$$\begin{aligned} L(\theta_1, a_1(0)) &= 1, & L(\theta_1, a_1(1)) &= 2, & L(\theta_1, a_2(0)) &= 4, & L(\theta_1, a_2(1)) &= 0; \\ L(\theta_2, a_1(0)) &= 3, & L(\theta_2, a_1(1)) &= 1, & L(\theta_2, a_2(0)) &= 1, & L(\theta_2, a_2(1)) &= 4. \end{aligned}$$

- (a) (5 pts) Suppose θ has the prior distribution $\Lambda(\theta)$ defined by $P(\theta = \theta_1) = 0.9$, $P(\theta = \theta_2) = 0.1$. What is the Bayes rule with respect to $\Lambda(\theta)$?
(b) (5 pts) Find the minimax rule(s).

Solution:

- (a) First, we compute the risks of each action, state pair.

$$\begin{aligned} R(\theta_1, a_1) &= \mathbb{E}_X[L(\theta_1, a_1) | \Theta = \theta_1] \\ &= P(X = 1 | \Theta = \theta_1) L(\theta_1, a_1(X = 1)) + P(X = 0 | \Theta = \theta_1) L(\theta_1, a_1(X = 0)) \\ &= 0.8 \times 2 + 0.2 \times 1 = 1.8, \end{aligned}$$

$$\begin{aligned} R(\theta_2, a_1) &= P(X = 1 | \Theta = \theta_2) L(\theta_2, a_1(X = 1)) + P(X = 0 | \Theta = \theta_2) L(\theta_2, a_1(X = 0)) \\ &= 0.6 \times 1 + 0.4 \times 3 = 1.8, \end{aligned}$$

$$\begin{aligned} R(\theta_1, a_2) &= P(X = 1 | \Theta = \theta_1) L(\theta_1, a_2(X = 1)) + P(X = 0 | \Theta = \theta_1) L(\theta_1, a_2(X = 0)) \\ &= 0.8 \times 0 + 0.2 \times 4 = 0.8, \end{aligned}$$

$$R(\theta_2, a_2) = 0.4 \times 1 + 0.6 \times 4 = 2.8.$$

Then,

$$BR(a_1) = (0.9, 0.1) \begin{pmatrix} 1.8 \\ 1.8 \end{pmatrix} = 1.8,$$

$$BR(a_2) = (0.9, 0.1) \begin{pmatrix} 0.8 \\ 2.8 \end{pmatrix} = 1.0.$$

Therefore the Bayes rule is a_2 .

(b)

$$\sup_{\theta \in \{\theta_1, \theta_2\}} R(\theta, a_1) = 1.8,$$

$$\sup_{\theta \in \{\theta_1, \theta_2\}} R(\theta, a_2) = 2.8.$$

Therefore, the minimax rule is a_1 .